@prefix : <http://finder.tuwien.ac.at/vocab/navigation#> .
@prefix cc: <http://creativecommons.org/ns#> .
@prefix rdfs: <http://www.w3.org/2000/01/rdf-schema#> .
@prefix dct: <http://purl.org/dc/terms/> .
@prefix ogc: <http://www.opengis.net/ont/geosparql#> .
@prefix owl: <http://www.w3.org/2002/07/owl#> .
@prefix rdf: <http://www.w3.org/1999/02/22-rdf-syntax-ns#> .
@prefix xml: <http://www.w3.org/XML/1998/namespace> .
@prefix xsd: <http://www.w3.org/2001/XMLSchema#> .
@prefix foaf: <http://xmlns.com/foaf/0.1/> .
@prefix vann: <http://purl.org/vocab/vann/> .
@prefix voaf: <http://purl.org/vocommons/voaf#> .

<http://finder.tuwien.ac.at/vocab/navigation#> a owl:Ontology ;
	owl:versionIRI :0.1-SNAPSHOT ;
	owl:imports <http://www.opengis.net/ont/geosparql> ;
	dct:modified "2016-15-11"@en ;
	dct:title "Ontology for modelling indoor navigation."@en ;
	dct:contributor <http://finder.tuwien.ac.at/person/id/Kevin_Haller> ;
	vann:preferredNamespacePrefix "navi" ;
	voaf:reliesOn <http://www.opengis.net/ont/geosparql#> ;
	dct:abstract "Diese Ontology dient zur Modellierung von Navigation im Inneren von Gebäuden."@de ;
	vann:preferredNamespaceUri "http://finder.tuwien.ac.at/vocab/navigation#"^^xsd:anyURI ;
	rdfs:label "Ontologie um Navigation im Inneren von Gebäuden zu modellieren."@de ;
	voaf:reliesOn <http://www.opengis.net/ont/geosparql> ;
	dct:abstract "This is an ontology for modelling indoor navigation."@en ;
	dct:title "Ontologie um Navigation im Inneren von Gebäuden zu modellieren."@de ;
	rdfs:label "Ontology for modelling indoor navigation."@en ;
	dct:created "2016-09-20"@en .
# 
# 
# ###############################
# #
# #    Object Properties
# #
# ###############################
# 
# 
# http://finder.tuwien.ac.at/vocab/navigation#accessTo

:accessTo a owl:ObjectProperty ;
	rdfs:domain :Access ;
	rdfs:range ogc:Feature ;
	rdfs:comment "Dieser Zugang bereitet Zugang zu einem oder mehreren räumlichen Features."@de ,
		"This access provides access to one or more given features."@en ;
	rdfs:isDefinedBy "http://finder.tuwien.ac.at/vocab/navigation#" ;
	rdfs:label "Zugang zu"@de , "access to"@en .
# 
# http://finder.tuwien.ac.at/vocab/navigation#hasContraint

:hasContraint a owl:ObjectProperty ;
	rdfs:domain :NavigationEntity ;
	rdfs:range :Constraint ;
	rdfs:comment "Diese Navigations-Entität hat die gegebene Beschränkung."@de ,
		"This navigation entity has the given constraint."@en ;
	rdfs:isDefinedBy "http://finder.tuwien.ac.at/vocab/navigation#" ;
	rdfs:label "has constraint"@en , "hat Beschränkung"@de .
# 
# http://finder.tuwien.ac.at/vocab/navigation#provideAccess

:provideAccess a owl:ObjectProperty ;
	rdfs:domain ogc:Feature ;
	rdfs:range :Access ;
	rdfs:comment "Dieses räumliche Feature bietet den gegebenen Zugang an."@de ,
		"This spatial feature provides an access."@en ;
	rdfs:isDefinedBy "http://finder.tuwien.ac.at/vocab/navigation#" ;
	rdfs:label "bietet Zugang an"@de , "provide access"@en .
# 
# http://finder.tuwien.ac.at/vocab/navigation#xFeature

:xFeature a owl:ObjectProperty ;
	owl:inverseOf :xOfRoute ;
	rdfs:domain :Route ;
	rdfs:range ogc:Feature ;
	rdfs:comment "Diese Route R(x,y) hat das gegebene räumliche Feature als Ausgangspunkt x."@de ,
		"This route R(x,y) has the given spatial feature as starting point x."@en ;
	rdfs:isDefinedBy "http://finder.tuwien.ac.at/vocab/navigation#" ;
	rdfs:label "Feature for x"@en , "Feature für x"@de .
# 
# http://finder.tuwien.ac.at/vocab/navigation#xOfRoute

:xOfRoute a owl:ObjectProperty ;
	rdfs:domain ogc:Feature ;
	rdfs:range :Route ;
	rdfs:comment "Dieses räumliche Feature ist der x-Punkt der gegebenen Strecke R(x,y)."@de ,
		"This spatial feature is the x point of the given route R(x, y),"@en ;
	rdfs:isDefinedBy "http://finder.tuwien.ac.at/vocab/navigation#" ;
	rdfs:label "x einer Strecke R(x,y)"@de , "x of a route R(x,y)"@en .
# 
# http://finder.tuwien.ac.at/vocab/navigation#xyFeature

:xyFeature a owl:ObjectProperty ;
	rdfs:subPropertyOf :xFeature , :yFeature ;
	owl:inverseOf :xyOfRoute ;
	rdfs:domain :BiRoute ;
	rdfs:range ogc:Feature ;
	rdfs:comment """Diese BiRoute R(x,y) hat das gegebene räumliche Feature als Start-
(x) und Endpunkt (y)."""@de ,
		"This biroute R(x,y) has the given spatial feature as starting (x) and end point (y)."@en ;
	rdfs:isDefinedBy "http://finder.tuwien.ac.at/vocab/navigation#" ;
	rdfs:label "Feature for x or y"@en , "Feature für x oder y"@de .
# 
# http://finder.tuwien.ac.at/vocab/navigation#xyOfRoute

:xyOfRoute a owl:ObjectProperty ;
	rdfs:subPropertyOf :xOfRoute , :yOfRoute ;
	rdfs:domain ogc:Feature ;
	rdfs:range :BiRoute ;
	rdfs:comment """Das räumliche Feature ist Teil der gegebenen BiRoute R(x,y).
Es kann entweder x oder y sein."""@de ,
		"This spatial feature is part of the given BiRoute R(x,y). It can be x and y of the Route."@en ;
	rdfs:isDefinedBy "http://finder.tuwien.ac.at/vocab/navigation#" ;
	rdfs:label "x oder y einer Route"@de , "x or y of a BiRoute"@en .
# 
# http://finder.tuwien.ac.at/vocab/navigation#yFeature

:yFeature a owl:ObjectProperty ;
	owl:inverseOf :yOfRoute ;
	rdfs:domain :Route ;
	rdfs:range ogc:Feature .
# 
# http://finder.tuwien.ac.at/vocab/navigation#yOfRoute

:yOfRoute a owl:ObjectProperty ;
	rdfs:domain ogc:Feature ;
	rdfs:range :Route .
# 
# 
# 
# ###############################
# #
# #    Classes
# #
# ###############################
# 
# 
# http://finder.tuwien.ac.at/vocab/navigation#Access

:Access a owl:Class ;
	rdfs:subClassOf :NavigationEntity ;
	rdfs:comment """Beschreibt einen Zugang zu gegebenen räumlichen Features unter Berücksichtigung
möglicher Beschränkungen."""@de ,
		"Describes the access to certain features by considering possible constraints."@en ;
	rdfs:isDefinedBy <http://finder.tuwien.ac.at/vocab/navigation#> ;
	rdfs:label "Access"@en , "Zugang"@de .
# 
# http://finder.tuwien.ac.at/vocab/navigation#BiRoute

:BiRoute a owl:Class ;
	rdfs:subClassOf :Route ;
	rdfs:comment """Beschreibt eine bidirektionale Strecke zwischen zwei räumlichen Features,
was bedeutet, dass die Strecke zwischen x und y in beide Richtungen begehbar ist mit den selben 
Eigenschaften und Einschränkungen."""@de , 
		"""Describes a bidirectional route between two spatial features, means that the route 
is walk-able from x to y and from y to x with the same constraints and characteristics."""@en ;
	rdfs:isDefinedBy <http://finder.tuwien.ac.at/vocab/navigation#> ;
	rdfs:label "Bidirectional Route"@en , "Bidirektionale Strecke"@de .
# 
# http://finder.tuwien.ac.at/vocab/navigation#Constraint

:Constraint a owl:Class ;
	owl:disjointWith :PoR , :Route ;
	rdfs:comment """A constraint for a navigation entity like access control, existing 
obstacles that are hard to overcome for persons with mobility impairments or opening hours."""@en , 
		"""Eine Beschränkung für eine Navigationsentität wie eine Zugangskontrolle, 
Hindernisse für Personen mit Mobilitätseinschränkungen oder Öffnungszeiten."""@de ;
	rdfs:isDefinedBy <http://finder.tuwien.ac.at/vocab/navigation#> ;
	rdfs:label "Beschränkung"@de , "Constraint"@en .
# 
# http://finder.tuwien.ac.at/vocab/navigation#MobilityConstraint

:MobilityConstraint a owl:Class ;
	rdfs:subClassOf :Constraint ;
	rdfs:comment """Beschreibt ein Hindernis, das Personen mit Mobilitätseinschränkungen 
betreffen könnte."""@de , 
		"Describes an obstacle that may affect persons with mobility impairments."@en ;
	rdfs:isDefinedBy <http://finder.tuwien.ac.at/vocab/navigation#> ;
	rdfs:label "Mobility constraints"@en , "Mobilitätseinschränkung"@de .
# 
# http://finder.tuwien.ac.at/vocab/navigation#NavigationEntity

:NavigationEntity a owl:Class ;
	rdfs:comment """Navigation entity is an entity important for navigation (e.g. a route
from one point to another)."@en ,
		"""Navigationsentität ist eine Entität für Navigationen (eine Route von einem Punkt
zum anderen)."""@de ;
	rdfs:isDefinedBy <http://finder.tuwien.ac.at/vocab/navigation#> ;
	rdfs:label "NavigationEntity"@en , "Navigationsentität"@de .
# 
# http://finder.tuwien.ac.at/vocab/navigation#PoR

:PoR a owl:Class ;
	rdfs:subClassOf ogc:Feature ;
	owl:disjointWith :Route ;
	rdfs:comment """Point of a route that is somehow interesting for a route, but does 
not have any further purpose."""@en ,
		"""Punkt einer Route, der irgendwie interessant für eine Route ist, aber darüber 
hinaus keine Funktion hat."""@de ;
	rdfs:isDefinedBy "http://finder.tuwien.ac.at/vocab/navigation#" ;
	rdfs:label "Point of Route"@en , "Punkt einer Route"@de .
# 
# http://finder.tuwien.ac.at/vocab/navigation#Route

:Route a owl:Class ;
	rdfs:subClassOf :NavigationEntity ;
	rdfs:comment """Beschreibt eine Strecke zwischen zwei raümlichen Features wie zum Beispiel
einem Eingang und einem Raum. R(x, y), wobei ein gehbarer Weg zwischen x und y besteht in 
genau dieser Richtung. Es werden keine Annahmen über die andere Richtung getroffen."""@de , 
		"""Describes a route between two spatial features such as between an entrance and an 
room. This route can have constraints for certain agents. R(x, y), where there is a walk-able 
path between x and y in exactly this direction. No assumption about the other direction 
are made."""@en ;
	rdfs:isDefinedBy <http://finder.tuwien.ac.at/vocab/navigation#> ;
	rdfs:label "Route"@en , "Strecke"@de .
# 
# http://finder.tuwien.ac.at/vocab/navigation#TimeConstraint

:TimeConstraint a owl:Class ;
	rdfs:subClassOf :Constraint ;
	rdfs:comment "A time constraint like opening hours for entrances to a building."@en ,
		"Eine Zeitbeschränkung wie Öffnungszeiten für Eingänge zu einem Gebäude."@de ;
	rdfs:isDefinedBy <http://finder.tuwien.ac.at/vocab/navigation#> ;
	rdfs:label "Time constraint"@en , "Zeitbeschränkung"@de .

# 
# 
# 
# ###############################
# #
# #    Individuals
# #
# ###############################
# 
# 
# http://finder.tuwien.ac.at/person/id/Kevin_Haller

<http://finder.tuwien.ac.at/person/id/Kevin_Haller> a owl:NamedIndividual , foaf:Person .
# 
# Generated by the OWL API (version 4.2.5.20160517-0735) https://github.com/owlcs/owlapi
